%%%%%%
%BASE
%%%
\documentclass[12pt,a4paper]{article}
\usepackage[utf8]{inputenc}
\usepackage[T1]{fontenc}
\usepackage[francais]{babel}

%%%%%
%MATHS
%%%
\usepackage{amsmath}
\usepackage{array}

%%%%%
%COULEURS
%%%
\usepackage{xcolor}
\usepackage{color}

%%%%%
%PUCES
%%%
\usepackage{pifont}

\everymath{\displaystyle}
\usepackage{hyperref}
\setlength{\parindent}{10px}

\usepackage{tikz,tkz-tab}


%%%%%
%Haut de Page
%%%
\usepackage{fancybox}
\usepackage{fancyhdr}
\usepackage[left=1.3cm,right=1.2cm,top=2cm,bottom=1.5cm]{geometry}
\pagestyle{fancy}
\fancyhead[L]{Lespinasse Florentin}
\fancyhead[C]{}
\fancyhead[R]{1STI2D4~~~~~~~~\today}

\begin{document}
\begin{center}
        \shadowbox{\begin{large}
                \textcolor{black}{17p239 }
        \end{large}}
    \end{center}
    \vspace{0.5 cm}

\begin{enumerate}
	\item	$f(x) = (2x-1)(x+4)$\par
			$u =		(2x-1)		v =		(x+4)$\par
			$u' =	2 			v' =	1	$\par
	$f'(x) = 2x+8 + 2x-1$\par
	$f'(x) = 4x+7$\par
    \vspace{0.5 cm}
	\item	$g(x) = x(5-3x)$\par
             $u =   x           v = (5-3x)    $\par
             $u' =   1           v' =   -3   $\par
     $f'(x) = 5-3x + (-3x)$\par
     $f'(x) = 5 - 6x$\par

\end{enumerate}

\begin{center}
        \shadowbox{\begin{large}
                \textcolor{black}{34p240 }
        \end{large}}
    \end{center}
    \vspace{0.5 cm}
\begin{enumerate}
     \item   $h(x) = x^2(3x+2)$\par
             $u =     x^2      v =     (3x+2)$\par
             $u' =   2x           v' =    3   $\par
     $f'(x) = 6x^2+4x + 3x^2$\par
     $f'(x) = 9x^2+4x$\par
     \vspace{0.5 cm}
     \item   $u(x) = (3x^2+2x-1)(2x-5)$\par
              $u =    (3x^2+2x-1) v = (2x-5)    $\par
              $u' =   (6x^2+2)    v' = 2   $\par
      $u'(x) = 12x^3 - 30x^2 + 4x - 10 + (6x^2 + 10x - 2)$\par
      $u'(x) = 12x^3 - 24x^2 + 14x - 12$\par
      
 \end{enumerate}




\end{document}

